aneris/examples/reliable_communication/spec/ras.v
@@ -4,39 +4,21 @@ From iris.algebra.lib Require Import excl_auth mono_nat.
 From iris.base_logic.lib Require Import mono_nat.
 From aneris.aneris_lang Require Import lang.
 From aneris.aneris_lang.lib Require Import lock_proof.
-
 From actris.channel Require Import proto.
 From aneris.examples.reliable_communication.spec Require Import prelude.
+From aneris.examples.reliable_communication.resources Require Import session_escrow.
 
 Definition session_names_mapUR : ucmra :=
   gmapUR socket_address (agreeR (leibnizO (session_name))).
 Definition session_names_map :=
   gmap socket_address (leibnizO (session_name)).
 
-Definition spec_chan_msg_history (A : ofe) :=
-  authUR (@monotoneUR (listO A) (prefix)).
-Notation SPrinCMH l := (principal prefix l).
-
-Class SpecChanMsgHist A Σ := {
-    SpecCMH_msghΣ :> inG Σ (spec_chan_msg_history A);
-    SpecCMH_msgcΣ :> inG Σ (frac_authR natR)
-  }.
-
-Definition SpecChanMsgHistΣ A : gFunctors :=
-  #[GFunctor (spec_chan_msg_history A);
-    GFunctor (frac_authR natR)].
-
-Global Instance SpecSubG_ChanMsgHistΣ A {Σ} :
-  subG (SpecChanMsgHistΣ A) Σ → SpecChanMsgHist A Σ.
-Proof. solve_inG. Qed.
-
 Notation socket_addressO := (leibnizO socket_address).
 
 Definition oneShotR := csumR (exclR unitO) (agreeR unitO).
 
 Class SpecChanG Σ := {
-    SpecChanG_proto :> protoG Σ val;
-    SpecChanG_chan_logbuf :> SpecChanMsgHist valO Σ;
+    SpecChanG_session_escrow :> session_escrowG Σ val;
     SpecChanG_ids :> mono_natG Σ;
     SpecChanG_cookie :> inG Σ (frac_authR natR);
     SpecChanG_session_names_map :>
@@ -50,8 +32,7 @@ Class SpecChanG Σ := {
    }.
 
 Definition SpecChanΣ : gFunctors :=
-  #[ protoΣ val;
-     SpecChanMsgHistΣ valO;
+  #[ session_escrowΣ val;
      mono_natΣ;
      GFunctor (frac_authR natR);
      GFunctor (authR (gmapUR socket_address (agreeR (leibnizO (session_name)))));
