aneris/aneris_lang/program_logic/step_update.v
@@ -1,0 +1,215 @@
+From iris.proofmode Require Import tactics.
+From aneris.aneris_lang.program_logic Require Import aneris_weakestpre.
+
+Section with_Σ.
+  Context `{!anerisG Mdl Σ}.
+
+  (* TODO: Move/Rename these *)
+  Lemma step_fupdN_frame_l' Eo Ei n (R Q : iProp Σ) :
+    (▷^n R ∗ |={Eo}[Ei]▷=>^n Q) -∗ |={Eo}[Ei]▷=>^n (R ∗ Q).
+  Proof.
+    induction n as [|n IH]; simpl; [done|].
+    iIntros "[HR HQ]".
+    iApply IH. by iFrame.
+  Qed.
+
+  Lemma step_fupdN_empty_sep n (R Q : iProp Σ) :
+    (|={∅}▷=>^n R) ∗ (|={∅}▷=>^n Q) -∗ |={∅}▷=>^n (R ∗ Q).
+  Proof.
+    induction n as [|n IH]; simpl; [done|].
+    iIntros "[HR HQ]". iApply IH.
+    iMod "HR". iMod "HQ". iIntros "!>!>". iMod "HR". iMod "HQ". by iFrame.
+  Qed.
+
+  Definition step_update E1 E2 P : iProp Σ :=
+    ∀ n, steps_auth n ={E1,E2}=∗
+         (steps_auth n ∗ (|={∅}▷=>^(S n) (steps_auth (S n) ={E2,E1}=∗
+                                          steps_auth (S n) ∗ P))).
+
+  Notation "|~{ E1 , E2 }~> P" := (step_update E1 E2 P) (at level 99, P at level 200, format "'[  ' |~{  E1  ,  E2  }~>  '/' P ']'").
+  Notation "|~{ E }~> P" := (step_update E ∅ P) (at level 99, P at level 200, format "'[  ' |~{  E  }~>  '/' P ']'").
+  Notation "|~~> P" := (|~{∅}~> P) (at level 99, P at level 200, format "'[  ' |~~>  '/' P ']'").
+
+  Lemma step_update_frame E1 E2 Ef P :
+    E2 ⊆ E1 → E1 ## Ef →
+    (|~{E1,E2}~> P) -∗
+    (|~{E1 ∪ Ef,E2 ∪ Ef}~> P).
+  Proof.
+    iIntros (Hle Hidjs) "Hstep".
+    iIntros (n) "Hauth".
+    iDestruct ("Hstep" with "Hauth") as "Hstep".
+    iDestruct (fupd_mask_frame_r E1 E2 Ef with "Hstep") as "Hstep"; [done|].
+    iMod "Hstep" as "[Hauth Hstep]".
+    iApply fupd_mask_intro; [done|].
+    iIntros "Hclose".
+    iFrame=> /=.
+    iMod "Hstep". iIntros "!>!>". iMod "Hstep". iIntros "!>".
+    iApply (step_fupdN_wand with "Hstep").
+    iIntros "Hstep Hauth".
+    iDestruct ("Hstep" with "Hauth") as "Hstep".
+    iMod "Hclose".
+    iApply fupd_mask_frame_r; [set_solver|].
+    iMod "Hstep".
+    iModIntro. done.
+  Qed.
+
+  Lemma aneris_wp_step_update_strong ip E1 E2 e P Φ :
+    TCEq (to_val e) None → E2 ⊆ E1 →
+    (|~{E1,E2}~> P) -∗
+    WP e @[ip] E2 {{ v, P ={E1}=∗ Φ v }} -∗
+    WP e @[ip] E1 {{ Φ }}.
+  Proof.
+    iIntros (Hval HE) "Hstep Hwp".
+    rewrite !aneris_wp_unfold /aneris_wp_def.
+    iIntros (tid) "Hip".
+    iDestruct ("Hwp" with "Hip") as "Hwp".
+    rewrite !wp_unfold /wp_pre /=.
+    rewrite /aneris_to_val. simpl. rewrite Hval. simpl.
+    iIntros (extr atr K tp1 tp2 σ1 Hexvalid Hloc Hexe)
+            "(?&?&?&?&Hauth)".
+    iMod ("Hstep" with "Hauth") as "[Hauth Hstep]". simpl.
+    iMod ("Hwp" with "[//] [//] [//] [$]") as "[% H]".
+    iMod "Hstep".
+    iModIntro.
+    iSplit; [done|].
+    iIntros (e2 σ2 efs Hstep). simpl.
+    iMod ("H" with "[//]") as "H". iIntros "!> !>".
+    iMod "H" as "H".
+    iMod "Hstep".
+    iIntros "!>".
+    iAssert (|={∅}▷=>^(trace_length extr) _ ∗ _)%I with "[H Hstep]" as "H".
+    { iApply step_fupdN_empty_sep. iFrame. }
+    iApply (step_fupdN_wand with "[H]"); first by iApply "H".
+    iIntros "[Hstep H]". iMod "H" as (δ2 ℓ) "((?&?&?&?&Hauth) & H & Hefs)".
+    iMod ("Hstep" with "Hauth") as "[Hauth HP]".
+    iModIntro.
+    iExists δ2, ℓ.
+    iFrame.
+    iApply (wp_strong_mono with "H"); [done|done|..].
+    iIntros (v) "H".
+    iDestruct "H" as (w Hw) "H".
+    iMod ("H" with "HP") as "H".
+    iModIntro. iExists _. iFrame. done.
+  Qed.
+
+  Lemma aneris_wp_step_update ip E1 E2 e P Φ :
+    TCEq (to_val e) None → E2 ⊆ E1 →
+    (|~{E1∖E2}~> P) -∗
+    WP e @[ip] E2 {{ v, P ={E1}=∗ Φ v }} -∗
+    WP e @[ip] E1 {{ Φ }}.
+  Proof.
+    iIntros (Hval HE) "Hstep Hwp".
+    iDestruct (step_update_frame (E1∖E2) ∅ (E2) with "Hstep") as "Hstep";
+      [set_solver|set_solver|].
+    replace (E1 ∖ E2 ∪ E2) with E1; last first.
+    { rewrite difference_union_L. set_solver. }
+    replace (∅ ∪ E2) with E2 by set_solver.
+    by iApply (aneris_wp_step_update_strong with "Hstep").
+  Qed.
+
+  Lemma step_update_frame_l E1 E2 P Q :
+    (|~{E1,E2}~> P) -∗ (|={E1}=> Q) -∗ |~{E1,E2}~> (P ∗ Q).
+  Proof.
+    iIntros "HP HQ" (n) "Hauth".
+    iMod "HQ". iMod ("HP" with "Hauth") as "[Hauth HP]".
+    iIntros "!>". iFrame=> /=.
+    iMod "HP". iIntros "!>!>". iMod "HP". iIntros "!>".
+    iApply (step_fupdN_wand with "HP").
+    iIntros "HP Hauth". iMod ("HP" with "Hauth") as "[Hauth HP]". by iFrame.
+  Qed.
+
+  Lemma step_update_comm P Q :
+    (|~~> P) -∗ (|~~> Q) -∗ |~~> P ∗ Q.
+  Proof.
+    iIntros "HP HQ" (n) "Hauth".
+    iMod ("HP" with "Hauth") as "[Hauth HP]".
+    iMod ("HQ" with "Hauth") as "[Hauth HQ]".
+    iIntros "!>". iFrame=> /=.
+    iMod "HP". iMod "HQ". iIntros "!>!>". iMod "HP". iMod "HQ". iIntros "!>".
+    iDestruct (step_fupdN_empty_sep with "[$HP $HQ]") as "HPQ".
+    iApply (step_fupdN_wand with "[HPQ]"); first by iApply "HPQ".
+    iIntros "[HP HQ] Hauth".
+    iMod ("HP" with "Hauth") as "[Hauth HP]".
+    iMod ("HQ" with "Hauth") as "[Hauth HQ]".
+    by iFrame.
+  Qed.
+
+  Lemma step_update_impl E1 E2 P Q :
+    (|~{E2,E2}~> P) -∗ (|~{E1,E2}~> P -∗ Q) -∗ |~{E1,E2}~> Q.
+  Proof.
+    iIntros "HP HPQ" (n) "Hauth".
+    iMod ("HPQ" with "Hauth") as "[Hauth HPQ]".
+    iMod ("HP" with "Hauth") as "[Hauth HP]".
+    iIntros "!>". iFrame=> /=.
+    iMod "HP". iMod "HPQ". iIntros "!>!>". iMod "HP". iMod "HPQ". iIntros "!>".
+    iAssert (|={∅}▷=>^n _ ∗ _)%I with "[HPQ HP]" as "H".
+    { iApply step_fupdN_empty_sep. iFrame. }
+    iApply (step_fupdN_wand with "H").
+    iIntros "[HP HPQ] Hauth".
+    iMod ("HP" with "Hauth") as "[Hauth HP]".
+    iMod ("HPQ" with "Hauth") as "[Hauth HPQ]".
+    iFrame. by iApply "HPQ".
+  Qed.
+
+  Lemma step_update_mono E1 E2 E3 P Q :
+    E2 ⊆ E1 → (|~{E2,E3}~> P) -∗ (P ={E2,E1}=∗ Q) -∗ |~{E1,E3}~> Q.
+  Proof.
+    iIntros (Hle) "HP HPQ". iIntros (n) "Hauth".
+    iApply fupd_mask_weaken; [done|]. iIntros "Hclose".
+    iMod ("HP" with "Hauth") as "[Hauth HP]".
+    iIntros "!>". iFrame=> /=.
+    iMod "HP". iIntros "!>!>". iMod "HP". iIntros "!>".
+    iAssert (|={∅}▷=>^n _ ∗ _)%I with "[HPQ HP]" as "H".
+    { iApply step_fupdN_frame_l. iFrame. iExact "HPQ". }
+    iApply (step_fupdN_wand with "H").
+    iIntros "[HPQ HP] Hauth".
+    iMod ("HP" with "Hauth") as "[Hauth HP]".
+    iMod ("HPQ" with "HP") as "HQ".
+    by iFrame.
+  Qed.
+
+  Lemma step_update_open E1 E2 E3 P :
+    (|={E1,E2}=> |~{E2,E3}~> (|={E2, E1}=> P)) -∗ |~{E1,E3}~> P.
+  Proof.
+    iIntros "Hstep" (n) "Hauth".
+    iMod "Hstep". iMod ("Hstep" with "Hauth") as "[Hauth Hstep]".
+    iIntros "!>". iFrame=> /=.
+    iMod "Hstep". iIntros "!>!>". iMod "Hstep". iIntros "!>".
+    iApply (step_fupdN_wand with "Hstep").
+    iIntros "Hstep Hauth".
+    iMod ("Hstep" with "Hauth") as "[Hauth Hstep]".
+    iMod "Hstep". iModIntro. by iFrame.
+  Qed.
+
+  Lemma step_update_lb_update E n :
+    steps_lb n -∗ |~{E}~> (steps_lb (S n)).
+  Proof.
+    iIntros "Hlb" (m) "Hauth".
+    iDestruct (steps_lb_valid with "Hauth Hlb") as %Hvalid.
+    iApply fupd_mask_intro; [set_solver|]. iIntros "Hclose". iFrame=> /=.
+    iIntros "!>!>!>".
+    iApply step_fupdN_intro; [done|].
+    iIntros "!> Hauth".
+    iDestruct (steps_lb_get with "Hauth") as "#Hlb'".
+    iDestruct (steps_lb_le _ (S n) with "Hlb'") as "Hlb''"; [lia|].
+    iMod "Hclose". iFrame. done.
+  Qed.
+
+  Lemma step_update_lb_step E P n :
+    steps_lb n -∗ (|={∅}▷=>^(S n) P) -∗ |~{E}~> P.
+  Proof.
+    iIntros "Hlb HP" (m) "Hauth".
+    iDestruct (steps_lb_valid with "Hauth Hlb") as %Hvalid.
+    iApply fupd_mask_intro; [set_solver|].
+    iIntros "Hclose". iFrame.
+    iApply (step_fupdN_le (S n)); [lia|done|].
+    iApply (step_fupdN_wand with "HP").
+    iIntros "HP Hauth".
+    iMod "Hclose". by iFrame.
+  Qed.
+
+End with_Σ.
+
+Notation "|~{ E1 , E2 }~> P" := (step_update E1 E2 P) (at level 99, P at level 200, format "'[  ' |~{  E1  ,  E2  }~>  '/' P ']'").
+Notation "|~{ E }~> P" := (step_update E ∅ P) (at level 99, P at level 200, format "'[  ' |~{  E  }~>  '/' P ']'").
+Notation "|~~> P" := (|~{∅}~> P) (at level 99, P at level 200, format "'[  ' |~~>  '/' P ']'").
