aneris/examples/reliable_communication/proof/common_user/proof_of_recv.v
@@ -7,7 +7,7 @@ From aneris.aneris_lang Require Import ast.
 From aneris.aneris_lang.lib.serialization Require Import serialization_proof.
 From aneris.aneris_lang.lib Require Import network_util_code.
 From aneris.aneris_lang.lib Require Import assert_proof lock_proof monitor_proof queue_proof.
-From aneris.aneris_lang.program_logic Require Import aneris_lifting.
+From aneris.aneris_lang.program_logic Require Import aneris_lifting step_update.
 From aneris.aneris_lang Require Import proofmode.
 From stdpp Require Import base tactics telescopes.
 From aneris.examples.reliable_communication Require Import client_server_code.
@@ -34,9 +34,9 @@ Section Proof_of_recv.
     iDestruct "Hc"
       as (sbuf slk rbuf rlk sidLBLoc ackIdLoc sidx ridx -> Heqc) "(%Heqg & Hc)".
     iDestruct "Hc"
-      as "(Hl & %Hleq & HT_at & HR_at & Hsidx & Hridx
+      as "(Hl & %Hleq & Hsidx & Hridx
                  & #HsnT & #HaT & #HsT & #HidxsT
-                 & Hp & #Hslk & #Hrlk & #Hinv)".
+                 & Hp & #Hslk & #Hrlk)".
     wp_lam.
     wp_pures.
     wp_apply (acquire_spec with "Hrlk").
@@ -53,15 +53,11 @@ Section Proof_of_recv.
       iLeft. iSplitR; [done|].
       iExists _, _, _, _, _, _, _, _.
       iExists _, _, _, _, _, _.
-      by iFrame "#∗"; eauto. }
+      iFrame. iFrame "#". eauto. }
     destruct Hqeq as (h & t & tv & -> & -> & Hq').
     iDestruct "Hvs" as "[(%w' & -> & Hfrag) Hvs]".
     wp_pures.
     wp_bind (Store _ _).
-    iInv (chan_N (endpoint_chan_name γe)) as "IH".
-    iDestruct "IH" as (Tl Tr Rl Rr) "(HTl & HTr & HRl & HRr & IH)".
-    iDestruct "IH" as "(>%Hpre1 & >%Hpre2 & Hlbl & Hlbr & Hctx)".
-    wp_store.
     iDestruct (mono_nat_auth_own_agree with "Hridx Hridx'") as %[_ <-].
     (* TODO: Fix weird split behaviour *)
     iMod (mono_nat_own_update (ridx + 1) with "[Hridx Hridx']")
@@ -69,123 +65,42 @@ Section Proof_of_recv.
       [|iApply fractional_half;
         [apply mono_nat_auth_own_as_fractional|iFrame]|]; [lia|].
     iDestruct "Hridx" as "[Hridx Hridx']".
-    destruct s => /=.
-    - iDestruct (auth_list_agree with "HTr Hfrag") as %Hnth.
-      iDestruct (auth_list_length with "HRl HR_at") as %Hlen.
-      rewrite -Hlen in Hnth.
-      rewrite Nat.add_0_r in Hnth.
-      rewrite (list_minus_alt Rl Tr); [|done].
-      rewrite (drop_S _ w'); [|done].
-      assert ((Rl ++ [w']) `prefix_of` Tr).
-      { destruct Hpre2 as [xs ->].
-        apply prefix_app.
-        rewrite lookup_app_r in Hnth; [|lia].
-        rewrite Nat.sub_diag in Hnth.
-        rewrite -head_lookup in Hnth.
-        destruct xs; [done|].
-        simpl in Hnth.
-        apply prefix_cons_alt; [|apply prefix_nil].
-        by inversion Hnth. }
-      iMod (iProto_recv_l with "Hctx Hp") as (p') "(Hctx & Hp &HP)".
-      iMod (auth_list_extend _ _ w' with "HRl HR_at") as "(HRl & HR_at & _)".
-      iModIntro.
-      iSplitL "HTl HTr HRl HRr Hlbl Hlbr Hctx".
-      { iNext.
-        iExists Tl, Tr, (Rl ++ [w']), Rr.
-        iFrame.
-        iSplit; [done|].
-        iSplit; [done|].
-        replace (S (length Rl)) with (length (Rl ++ [w'])); last first.
-        { rewrite app_length /=. lia. }
-        by rewrite -(list_minus_alt (Rl ++ [w']) Tr). }
-      wp_pures.
-      wp_apply (release_spec with "[$Hrlk $Hlocked Hrbuf HackIdLoc Hvs Hridx']").
-      { iExists _, _, _. iFrame. iSplit; [done|]. simpl.
-        rewrite !Nat.add_1_r.
-        rewrite -!Nat2Z.inj_add.
-        rewrite -Nat.add_succ_comm.
-        iFrame.
-        iApply (big_sepL_impl with "Hvs").
-        iIntros "!>" (k x Hlookup) "Hv".
-        rewrite Nat.add_succ_comm.
-        rewrite -!Nat2Z.inj_add.
-        rewrite -Nat.add_succ_comm.
-        done. }
-      iIntros (w'' ->).
-      iPoseProof (iMsg_texist_exist with "HP") as (x) "HP".
-      rewrite iMsg_base_eq /=.
-      wp_pures.
-      iApply "HΦ".
-      iRight.
-      iDestruct "HP" as "(%Heq'' & Hp' & HP)".
-      rewrite -Heq''.
-      iExists _. iSplit; [done|].
+    replace (ridx + 0) with ridx by lia.
+    iApply (aneris_wp_step_update _ _ ∅ with "[Hp Hfrag]");
+      [done|by iApply (step_update_recv with "Hp Hfrag")|].
+    wp_store.
+    iDestruct 1 as (p') "[Hp HP]".
+    iModIntro.
+    wp_pures.
+    wp_apply (release_spec with "[$Hrlk $Hlocked Hrbuf HackIdLoc Hvs Hridx']").
+    { iExists _, _, _. iFrame. iSplit; [done|]. simpl.
+      rewrite !Nat.add_1_r.
+      rewrite -!Nat2Z.inj_add.
+      rewrite -Nat.add_succ_comm.
       iFrame.
-      iExists _, _, _, _, _, _, _, _.
-      iExists _, _, _, _, _, _.
-      iSplit; [done|].
-      iRewrite "Hp'".
-      iFrame "#∗".
-      rewrite Nat.add_1_r.
-      eauto.
-    - iDestruct (auth_list_agree with "HTl Hfrag") as %Hnth.
-      iDestruct (auth_list_length with "HRr HR_at") as %Hlen.
-      rewrite -Hlen in Hnth.
-      rewrite Nat.add_0_r in Hnth.
-      rewrite (list_minus_alt Rr Tl); [|done].
-      rewrite (drop_S _ w'); [|done].
-      assert ((Rr ++ [w']) `prefix_of` Tl).
-      { destruct Hpre1 as [xs ->].
-        apply prefix_app.
-        rewrite lookup_app_r in Hnth; [|lia].
-        rewrite Nat.sub_diag in Hnth.
-        rewrite -head_lookup in Hnth.
-        destruct xs; [done|].
-        simpl in Hnth.
-        apply prefix_cons_alt; [|apply prefix_nil].
-        by inversion Hnth. }
-      iMod (iProto_recv_r with "Hctx Hp") as (p') "(Hctx & Hp &HP)".
-      iMod (auth_list_extend _ _ w' with "HRr HR_at") as "(HRr & HR_at & _)".
-      iModIntro.
-      iSplitL "HTl HTr HRl HRr Hlbl Hlbr Hctx".
-      { iNext.
-        iExists Tl, Tr, Rl, (Rr ++ [w']).
-        iFrame.
-        iSplit; [done|].
-        iSplit; [done|].
-        replace (S (length Rr)) with (length (Rr ++ [w'])); last first.
-        { rewrite app_length /=. lia. }
-        by rewrite -(list_minus_alt (Rr ++ [w']) Tl). }
-      wp_pures.
-      wp_apply (release_spec with "[$Hrlk $Hlocked Hrbuf HackIdLoc Hvs Hridx']").
-      { iExists _, _, _. iFrame. iSplit; [done|]. simpl.
-        rewrite !Nat.add_1_r.
-        rewrite -!Nat2Z.inj_add.
-        rewrite -Nat.add_succ_comm.
-        iFrame.
-        iApply (big_sepL_impl with "Hvs").
-        iIntros "!>" (k x Hlookup) "Hv".
-        rewrite Nat.add_succ_comm.
-        rewrite -!Nat2Z.inj_add.
-        rewrite -Nat.add_succ_comm.
-        done. }
-      iIntros (w'' ->).
-      iPoseProof (iMsg_texist_exist with "HP") as (x) "HP".
-      rewrite iMsg_base_eq /=.
-      wp_pures.
-      iApply "HΦ".
-      iRight.
-      iDestruct "HP" as "(%Heq'' & Hp' & HP)".
-      rewrite -Heq''.
-      iExists _. iSplit; [done|].
-      iFrame.
-      iExists _, _, _, _, _, _, _, _.
-      iExists _, _, _, _, _, _.
-      iSplit; [done|].
-      iRewrite "Hp'".
-      iFrame "#∗".
-      rewrite Nat.add_1_r.
-      eauto.
+      iApply (big_sepL_impl with "Hvs").
+      iIntros "!>" (k x Hlookup) "Hv".
+      rewrite Nat.add_succ_comm.
+      rewrite -!Nat2Z.inj_add.
+      rewrite -Nat.add_succ_comm.
+      done. }
+    iIntros (w'' ->).
+    iPoseProof (iMsg_texist_exist with "HP") as (x) "HP".
+    rewrite iMsg_base_eq /=.
+    wp_pures.
+    iApply "HΦ".
+    iRight.
+    iDestruct "HP" as "(%Heq'' & Hp' & HP)".
+    rewrite -Heq''.
+    iExists _. iSplit; [done|].
+    iFrame.
+    iExists _, _, _, _, _, _, _, _.
+    iExists _, _, _, _, _, _.
+    iSplit; [done|].
+    rewrite Nat.add_1_r.
+    iFrame=> /=.
+    iRewrite "Hp'".
+    iFrame. by iFrame "#".
   Qed.
 
   Lemma recv_spec_internal {TT} γe c (v : TT → val) (P : TT → iProp Σ)
