aneris/examples/reliable_communication/resources/mono_list.v
@@ -1,0 +1,204 @@
+(** OBS!: This is taken directly from Iris, and should instead be obtained
+from bumping the Iris version. *)
+
+(** Authoritative CMRA of append-only lists, where the fragment represents a
+  snap-shot of the list, and the authoritative element can only grow by
+  appending. *)
+From iris.algebra Require Export auth dfrac max_prefix_list.
+From iris.algebra Require Import updates local_updates proofmode_classes.
+From iris.prelude Require Import options.
+
+Definition mono_listR (A : ofe) : cmra  := authR (max_prefix_listUR A).
+Definition mono_listUR (A : ofe) : ucmra  := authUR (max_prefix_listUR A).
+
+Definition mono_list_auth {A : ofe} (q : dfrac) (l : list A) : mono_listR A :=
+  ●{q} (to_max_prefix_list l) ⋅ ◯ (to_max_prefix_list l).
+Definition mono_list_lb {A : ofe} (l : list A) : mono_listR A :=
+  ◯ (to_max_prefix_list l).
+Global Instance: Params (@mono_list_auth) 2 := {}.
+Global Instance: Params (@mono_list_lb) 1 := {}.
+Typeclasses Opaque mono_list_auth mono_list_lb.
+
+(** FIXME: Refactor these notations using custom entries once Coq bug #13654
+has been fixed. *)
+Notation "●ML{ dq } l" :=
+  (mono_list_auth dq l) (at level 20, format "●ML{ dq }  l").
+Notation "●ML{# q } l" :=
+  (mono_list_auth (DfracOwn q) l) (at level 20, format "●ML{# q }  l").
+Notation "●ML□ l" := (mono_list_auth DfracDiscarded l) (at level 20).
+Notation "●ML l" := (mono_list_auth (DfracOwn 1) l) (at level 20).
+Notation "◯ML l" := (mono_list_lb l) (at level 20).
+
+Section mono_list_props.
+  Context {A : ofe}.
+  Implicit Types l : list A.
+  Implicit Types q : frac.
+  Implicit Types dq : dfrac.
+
+  (** Setoid properties *)
+  Global Instance mono_list_auth_ne dq : NonExpansive (@mono_list_auth A dq).
+  Proof. solve_proper. Qed.
+  Global Instance mono_list_auth_proper dq : Proper ((≡) ==> (≡)) (@mono_list_auth A dq).
+  Proof. solve_proper. Qed.
+  Global Instance mono_list_lb_ne : NonExpansive (@mono_list_lb A).
+  Proof. solve_proper. Qed.
+  Global Instance mono_list_lb_proper : Proper ((≡) ==> (≡)) (@mono_list_lb A).
+  Proof. solve_proper. Qed.
+
+  Global Instance mono_list_lb_dist_inj n : Inj (dist n) (dist n) (@mono_list_lb A).
+  Proof. rewrite /mono_list_lb. by intros ?? ?%(inj _)%(inj _). Qed.
+  Global Instance mono_list_lb_inj : Inj (≡) (≡) (@mono_list_lb A).
+  Proof. rewrite /mono_list_lb. by intros ?? ?%(inj _)%(inj _). Qed.
+
+  (** * Operation *)
+  Global Instance mono_list_lb_core_id l : CoreId (◯ML l).
+  Proof. rewrite /mono_list_lb. apply _. Qed.
+  Global Instance mono_list_auth_core_id l : CoreId (●ML□ l).
+  Proof. rewrite /mono_list_auth. apply _. Qed.
+
+  Lemma mono_list_auth_dfrac_op dq1 dq2 l :
+    ●ML{dq1 ⋅ dq2} l ≡ ●ML{dq1} l ⋅ ●ML{dq2} l.
+  Proof.
+    rewrite /mono_list_auth auth_auth_dfrac_op.
+    rewrite (comm _ (●{dq2} _)) -!assoc (assoc _ (◯ _)).
+    by rewrite -core_id_dup (comm _ (◯ _)).
+  Qed.
+
+  Lemma mono_list_lb_op_l l1 l2 : l1 `prefix_of` l2 → ◯ML l1 ⋅ ◯ML l2 ≡ ◯ML l2.
+  Proof. intros ?. by rewrite /mono_list_lb -auth_frag_op to_max_prefix_list_op_l. Qed.
+  Lemma mono_list_lb_op_r l1 l2 : l1 `prefix_of` l2 → ◯ML l2 ⋅ ◯ML l1 ≡ ◯ML l2.
+  Proof. intros ?. by rewrite /mono_list_lb -auth_frag_op to_max_prefix_list_op_r. Qed.
+  Lemma mono_list_auth_lb_op dq l : ●ML{dq} l ≡ ●ML{dq} l ⋅ ◯ML l.
+  Proof.
+    by rewrite /mono_list_auth /mono_list_lb -!assoc -auth_frag_op -core_id_dup.
+  Qed.
+
+  Global Instance mono_list_auth_dfrac_is_op dq dq1 dq2 l :
+    IsOp dq dq1 dq2 → IsOp' (●ML{dq} l) (●ML{dq1} l) (●ML{dq2} l).
+  Proof. rewrite /IsOp' /IsOp=> ->. rewrite mono_list_auth_dfrac_op //. Qed.
+
+  (** * Validity *)
+  Lemma mono_list_auth_dfrac_validN n dq l : ✓{n} (●ML{dq} l) ↔ ✓ dq.
+  Proof.
+    rewrite /mono_list_auth auth_both_dfrac_validN.
+    naive_solver apply to_max_prefix_list_validN.
+  Qed.
+  Lemma mono_list_auth_validN n l : ✓{n} (●ML l).
+  Proof. by apply mono_list_auth_dfrac_validN. Qed.
+
+  Lemma mono_list_auth_dfrac_valid dq l : ✓ (●ML{dq} l) ↔ ✓ dq.
+  Proof.
+    rewrite /mono_list_auth auth_both_dfrac_valid.
+    naive_solver apply to_max_prefix_list_valid.
+  Qed.
+  Lemma mono_list_auth_valid l : ✓ (●ML l).
+  Proof. by apply mono_list_auth_dfrac_valid. Qed.
+
+  Lemma mono_list_auth_dfrac_op_validN n dq1 dq2 l1 l2 :
+    ✓{n} (●ML{dq1} l1 ⋅ ●ML{dq2} l2) ↔ ✓ (dq1 ⋅ dq2) ∧ l1 ≡{n}≡ l2.
+  Proof.
+    rewrite /mono_list_auth (comm _ (●{dq2} _)) -!assoc (assoc _ (◯ _)).
+    rewrite -auth_frag_op (comm _ (◯ _)) assoc. split.
+    - move=> /cmra_validN_op_l /auth_auth_dfrac_op_validN.
+      rewrite (inj_iff to_max_prefix_list). naive_solver.
+    - intros [? ->]. rewrite -core_id_dup -auth_auth_dfrac_op auth_both_dfrac_validN.
+      naive_solver apply to_max_prefix_list_validN.
+  Qed.
+  Lemma mono_list_auth_op_validN n l1 l2 : ✓{n} (●ML l1 ⋅ ●ML l2) ↔ False.
+  Proof. rewrite mono_list_auth_dfrac_op_validN. naive_solver. Qed.
+
+  Lemma mono_list_auth_dfrac_op_valid dq1 dq2 l1 l2 :
+    ✓ (●ML{dq1} l1 ⋅ ●ML{dq2} l2) ↔ ✓ (dq1 ⋅ dq2) ∧ l1 ≡ l2.
+  Proof.
+    rewrite cmra_valid_validN equiv_dist.
+    setoid_rewrite mono_list_auth_dfrac_op_validN. naive_solver eauto using O.
+  Qed.
+  Lemma mono_list_auth_op_valid l1 l2 : ✓ (●ML l1 ⋅ ●ML l2) ↔ False.
+  Proof. rewrite mono_list_auth_dfrac_op_valid. naive_solver. Qed.
+
+  Lemma mono_list_auth_dfrac_op_valid_L `{!LeibnizEquiv A} dq1 dq2 l1 l2 :
+    ✓ (●ML{dq1} l1 ⋅ ●ML{dq2} l2) ↔ ✓ (dq1 ⋅ dq2) ∧ l1 = l2.
+  Proof. unfold_leibniz. apply mono_list_auth_dfrac_op_valid. Qed.
+
+  Lemma mono_list_both_dfrac_validN n dq l1 l2 :
+    ✓{n} (●ML{dq} l1 ⋅ ◯ML l2) ↔ ✓ dq ∧ ∃ l, l1 ≡{n}≡ l2 ++ l.
+  Proof.
+    rewrite /mono_list_auth /mono_list_lb -assoc
+      -auth_frag_op auth_both_dfrac_validN -to_max_prefix_list_includedN.
+    f_equiv; split.
+    - intros [Hincl _]. etrans; [apply: cmra_includedN_r|done].
+    - intros. split; [|by apply to_max_prefix_list_validN].
+      rewrite {2}(core_id_dup (to_max_prefix_list l1)). by f_equiv.
+  Qed.
+  Lemma mono_list_both_validN n l1 l2 :
+    ✓{n} (●ML l1 ⋅ ◯ML l2) ↔ ∃ l, l1 ≡{n}≡ l2 ++ l.
+  Proof. rewrite mono_list_both_dfrac_validN. split; [naive_solver|done]. Qed.
+
+  Lemma mono_list_both_dfrac_valid dq l1 l2 :
+    ✓ (●ML{dq} l1 ⋅ ◯ML l2) ↔ ✓ dq ∧ ∃ l, l1 ≡ l2 ++ l.
+  Proof.
+    rewrite /mono_list_auth /mono_list_lb -assoc -auth_frag_op
+      auth_both_dfrac_valid -max_prefix_list_included_includedN
+      -to_max_prefix_list_included.
+    f_equiv; split.
+    - intros [Hincl _]. etrans; [apply: cmra_included_r|done].
+    - intros. split; [|by apply to_max_prefix_list_valid].
+      rewrite {2}(core_id_dup (to_max_prefix_list l1)). by f_equiv.
+  Qed.
+  Lemma mono_list_both_valid l1 l2 :
+    ✓ (●ML l1 ⋅ ◯ML l2) ↔ ∃ l, l1 ≡ l2 ++ l.
+  Proof. rewrite mono_list_both_dfrac_valid. split; [naive_solver|done]. Qed.
+
+  Lemma mono_list_both_dfrac_valid_L `{!LeibnizEquiv A} dq l1 l2 :
+    ✓ (●ML{dq} l1 ⋅ ◯ML l2) ↔ ✓ dq ∧ l2 `prefix_of` l1.
+  Proof. rewrite /prefix. rewrite mono_list_both_dfrac_valid. naive_solver. Qed.
+  Lemma mono_list_both_valid_L `{!LeibnizEquiv A} l1 l2 :
+    ✓ (●ML l1 ⋅ ◯ML l2) ↔ l2 `prefix_of` l1.
+  Proof. rewrite /prefix. rewrite mono_list_both_valid. naive_solver. Qed.
+
+  Lemma mono_list_lb_op_validN n l1 l2 :
+    ✓{n} (◯ML l1 ⋅ ◯ML l2) ↔ (∃ l, l2 ≡{n}≡ l1 ++ l) ∨ (∃ l, l1 ≡{n}≡ l2 ++ l).
+  Proof. by rewrite auth_frag_op_validN to_max_prefix_list_op_validN. Qed.
+  Lemma mono_list_lb_op_valid l1 l2 :
+    ✓ (◯ML l1 ⋅ ◯ML l2) ↔ (∃ l, l2 ≡ l1 ++ l) ∨ (∃ l, l1 ≡ l2 ++ l).
+  Proof. by rewrite auth_frag_op_valid to_max_prefix_list_op_valid. Qed.
+  Lemma mono_list_lb_op_valid_L `{!LeibnizEquiv A} l1 l2 :
+    ✓ (◯ML l1 ⋅ ◯ML l2) ↔ l1 `prefix_of` l2 ∨ l2 `prefix_of` l1.
+  Proof. rewrite mono_list_lb_op_valid / prefix. naive_solver. Qed.
+
+  Lemma mono_list_lb_op_valid_1_L `{!LeibnizEquiv A} l1 l2 :
+    ✓ (◯ML l1 ⋅ ◯ML l2) → l1 `prefix_of` l2 ∨ l2 `prefix_of` l1.
+  Proof. by apply mono_list_lb_op_valid_L. Qed.
+  Lemma mono_list_lb_op_valid_2_L `{!LeibnizEquiv A} l1 l2 :
+    l1 `prefix_of` l2 ∨ l2 `prefix_of` l1 → ✓ (◯ML l1 ⋅ ◯ML l2).
+  Proof. by apply mono_list_lb_op_valid_L. Qed.
+
+  Lemma mono_list_lb_mono l1 l2 : l1 `prefix_of` l2 → ◯ML l1 ≼ ◯ML l2.
+  Proof. intros. exists (◯ML l2). by rewrite mono_list_lb_op_l. Qed.
+
+  Lemma mono_list_included dq l : ◯ML l ≼ ●ML{dq} l.
+  Proof. apply cmra_included_r. Qed.
+
+  (** * Update *)
+  Lemma mono_list_update {l1} l2 : l1 `prefix_of` l2 → ●ML l1 ~~> ●ML l2.
+  Proof. intros ?. by apply auth_update, max_prefix_list_local_update. Qed.
+  Lemma mono_list_auth_persist dq l : ●ML{dq} l ~~> ●ML□ l.
+  Proof.
+    rewrite /mono_list_auth. apply cmra_update_op; [|done].
+    by apply auth_update_auth_persist.
+  Qed.
+End mono_list_props.
+
+Definition mono_listURF (F : oFunctor) : urFunctor :=
+  authURF (max_prefix_listURF F).
+
+Global Instance mono_listURF_contractive F :
+  oFunctorContractive F → urFunctorContractive (mono_listURF F).
+Proof. apply _. Qed.
+
+Definition mono_listRF (F : oFunctor) : rFunctor :=
+  authRF (max_prefix_listURF F).
+
+Global Instance mono_listRF_contractive F :
+  oFunctorContractive F → rFunctorContractive (mono_listRF F).
+Proof. apply _. Qed.
