aneris/examples/reliable_communication/resources/session_escrow.v
@@ -1,0 +1,359 @@
+From iris.algebra Require Import agree gmap auth excl numbers frac_auth csum.
+From iris.algebra.lib Require Import excl_auth mono_nat.
+From iris.base_logic.lib Require Import invariants mono_nat.
+From iris.proofmode Require Import tactics.
+From aneris.aneris_lang Require Import resources.
+From aneris.examples.reliable_communication.resources Require Export mono_list.
+From actris.channel Require Import proto.
+From aneris.aneris_lang.program_logic Require Import aneris_weakestpre step_update.
+From iris.bi Require Import updates.
+From aneris.aneris_lang.state_interp Require Import state_interp_def.
+
+Set Default Proof Using "Type".
+
+(** Side switch. *)
+Definition dual_side (s : side) : side := side_elim s Right Left.
+
+Record session_escrow_name :=
+  SessionEscrowName {
+      session_escrow_proto_name : proto_name;
+      session_escrow_Tl_name : gname;
+      session_escrow_Tr_name : gname;
+      session_escrow_sl_name : gname;
+      session_escrow_rl_name : gname;
+      session_escrow_sr_name : gname;
+      session_escrow_rr_name : gname
+    }.
+
+Global Instance session_escrow_name_inhabited : Inhabited session_escrow_name :=
+  populate (SessionEscrowName inhabitant inhabitant inhabitant inhabitant inhabitant inhabitant inhabitant).
+Global Instance session_escrow_name_eq_dec : EqDecision session_escrow_name.
+Proof. solve_decision. Qed.
+Global Instance session_escrow_name_countable : Countable session_escrow_name.
+Proof.
+  refine (inj_countable
+            (λ '(SessionEscrowName γp γ_Tl γ_Rl γ_sl γ_rl γ_sr γ_rr),
+               (γp, γ_Tl, γ_Rl, γ_sl, γ_rl, γ_sr, γ_rr))
+            (λ '(γp, γ_Tl, γ_Rl, γ_sl, γ_rl, γ_sr, γ_rr),
+               Some (SessionEscrowName γp γ_Tl γ_Rl γ_sl γ_rl γ_sr γ_rr)) _);
+    by intros [].
+Qed.
+
+Class session_escrowG Σ V := {
+    session_escrowG_protoG :> protoG Σ V;
+    session_escrowG_histG :> inG Σ (mono_listUR (leibnizO V));
+    session_escrowG_counterG :> inG Σ (excl_authR natO);
+  }.
+
+Definition session_escrowΣ V : gFunctors :=
+  #[protoΣ V; GFunctor (mono_listUR (leibnizO V)); GFunctor (excl_authR natO)].
+
+Global Instance subG_session_escrowΣ V {Σ} :
+  subG (session_escrowΣ V) Σ → session_escrowG Σ V.
+Proof. solve_inG. Qed.
+
+Section iProto_sessions.
+  Context `{A : Type}.
+  Context `{!session_escrowG Σ A, !anerisG Mdl Σ}.
+  Context (N : namespace).
+
+  Parameter γc : proto_name.
+  Parameter γTl : gname.
+  Parameter γTr : gname.
+  Parameter γsl : gname.
+  Parameter γrl : gname.
+  Parameter γsr : gname.
+  Parameter γrr : gname.
+
+  Definition auth_list (χ : session_escrow_name) (s : side) (xs : list A) :=
+    own (side_elim s (χ.(session_escrow_Tl_name)) (χ.(session_escrow_Tr_name)))
+        (●ML (xs : list (leibnizO A))).
+  Definition frag_list (χ : session_escrow_name) (s : side) (n : nat) (x : A) : iProp Σ :=
+    ∃ xs, ⌜xs !! n = Some x⌝ ∗
+          own (side_elim s (χ.(session_escrow_Tl_name))
+                         (χ.(session_escrow_Tr_name)))
+              (◯ML (xs : list (leibnizO A))).
+
+Definition auth_auth_sent (χ : session_escrow_name) (s : side) (n : nat) : iProp Σ :=
+    own (side_elim s χ.(session_escrow_sl_name) χ.(session_escrow_sr_name))
+        (●E n).
+  Definition auth_frag_sent (χ : session_escrow_name) (s : side) (n : nat) : iProp Σ :=
+    own (side_elim s χ.(session_escrow_sl_name) χ.(session_escrow_sr_name))
+        (◯E n).
+  Definition auth_auth_recv (χ : session_escrow_name) (s : side) (n : nat) : iProp Σ :=
+    own (side_elim s χ.(session_escrow_rl_name) χ.(session_escrow_rr_name))
+        (●E n).
+  Definition auth_frag_recv (χ : session_escrow_name) (s : side) (n : nat) : iProp Σ :=
+    own (side_elim s χ.(session_escrow_rl_name) χ.(session_escrow_rr_name))
+        (◯E n).
+
+  Definition Ses_inv (χ : session_escrow_name) : iProp Σ :=
+    ∃ (Tl Tr : list A) (nl nr : nat),
+      ⌜nr ≤ length Tl⌝ ∗ ⌜nl ≤ length Tr⌝ ∗
+      iProto_ctx χ.(session_escrow_proto_name) (drop nr Tl) (drop nl Tr) ∗
+      auth_list χ Left Tl ∗ auth_list χ Right Tr ∗
+      auth_auth_sent χ Left (length Tl) ∗ auth_auth_recv χ Left nl ∗
+      auth_auth_sent χ Right (length Tr) ∗ auth_auth_recv χ Right nr ∗
+      steps_lb (length Tl) ∗ steps_lb (length Tr).
+
+  Definition Ses (χ : session_escrow_name) : iProp Σ :=
+    inv N (Ses_inv χ).
+
+  Definition ses_own (χ : session_escrow_name) (s : side) (n m : nat) (p : iProto Σ A) : iProp Σ :=
+    Ses χ ∗
+    iProto_own χ.(session_escrow_proto_name) s p ∗
+    auth_frag_sent χ s n ∗ auth_frag_recv χ s m.
+
+  Global Instance ses_own_contractive χ s n m : Contractive (ses_own χ s n m).
+  Proof. solve_contractive. Qed.
+  Global Instance ses_own_ne χ s n m : NonExpansive (ses_own χ s n m).
+  Proof. solve_proper. Qed.
+  Global Instance ses_own_proper χ s n m : Proper ((≡) ==> (≡)) (ses_own χ s n m).
+  Proof. solve_proper. Qed.
+
+  Definition ses_idx (χ : session_escrow_name) (s : side) (n : nat) (x : A) :=
+    frag_list χ s n x.
+
+  Global Instance ses_idx_contractive χ s n v : Persistent (ses_idx χ s n v).
+  Proof. apply _. Qed.
+
+  Lemma ses_own_le χ s n m p1 p2 :
+    ses_own χ s n m p1 -∗ ▷ (p1 ⊑ p2) -∗ ses_own χ s n m p2.
+  Proof.
+    iIntros "(Hinv & Hp & H) Hle".
+    iDestruct (iProto_own_le with "Hp Hle") as "Hp". by iFrame.
+  Qed.
+
+  Lemma Ses_init E p :
+    ⊢ steps_lb 0 ={E}=∗
+          ∃ χ, Ses χ ∗ ses_own χ Left 0 0 p ∗ ses_own χ Right 0 0 (iProto_dual p).
+  Proof.
+    iIntros "#Hsteps".
+    iMod (iProto_init p) as (γc) "(Hctx & Hpl & Hpr)".
+    iMod (own_alloc (●ML [])) as (γl) "Hl"; [apply mono_list_auth_valid|].
+    iMod (own_alloc (●ML [])) as (γr) "Hr"; [apply mono_list_auth_valid|].
+    iMod (own_alloc (●E 0%nat ⋅ ◯E 0%nat)) as (γsl) "[HslA HslF]"; [apply excl_auth_valid|].
+    iMod (own_alloc (●E 0%nat ⋅ ◯E 0%nat)) as (γrl) "[HrlA HrlF]"; [apply excl_auth_valid|].
+    iMod (own_alloc (●E 0%nat ⋅ ◯E 0%nat)) as (γsr) "[HsrA HsrF]"; [apply excl_auth_valid|].
+    iMod (own_alloc (●E 0%nat ⋅ ◯E 0%nat)) as (γrr) "[HrrA HrrF]"; [apply excl_auth_valid|].
+    set (χ := SessionEscrowName γc γl γr γsl γrl γsr γrr).
+    iMod (inv_alloc N E (Ses_inv χ) with "[Hctx Hl Hr HslA HrlA HsrA HrrA]")
+      as "#H".
+    { iIntros "!>". iExists [], [], 0%nat, 0%nat. iFrame "#∗".
+      iSplit; iPureIntro; lia. }
+    iModIntro.
+    iExists χ.
+    iFrame "#∗".
+  Qed.
+
+  Lemma step_update_send_l χ E n m pm v p :
+    ↑N ⊆ E →
+    ses_own χ Left n m (<!> pm)%proto -∗ iMsg_car pm v (Next p) -∗
+    |~{E}~> (ses_own χ Left (S n) m p ∗ ses_idx χ Left n v).
+  Proof.
+    iIntros (HE) "[#HI (Hp&HslF&HrlF)] Hpm".
+    iApply step_update_open.
+    iInv N as "H" "Hclose".
+    iDestruct "H" as (Tl Tr nl nr)
+                       "(>%Hle&>%Hle2&Hctx&>HTl&>HTr&
+                       >Hsl&>Hrl&>Hsr&>Hrr&#>HTllb&#>HTrlb)".
+    iApply step_update_impl; [iApply step_update_lb_update; iApply "HTllb"|].
+    iApply step_update_lb_step; [iApply "HTrlb"|]=> /=.
+    iIntros "!>!>!>".
+    iMod (iProto_send_l with "Hctx Hp Hpm") as "[Hctx Hp]".
+    iModIntro.
+    iApply step_fupdN_intro; [done|].
+    iApply (bi.laterN_le (length (drop nl Tr))); [rewrite drop_length; lia|].
+    iIntros "!> #HTllb'".
+    iDestruct (own_valid_2 with "Hsl HslF") as %Hvalid1%excl_auth_agree_L.
+    iDestruct (own_valid_2 with "Hrl HrlF") as %Hvalid2%excl_auth_agree_L.
+    iMod (own_update_2 _ _ _ (●E (S (length Tl)) ⋅ ◯E (S (length Tl)))
+           with "Hsl HslF") as "[Hsl HslF]"; [by apply excl_auth_update|].
+    iMod (own_update _ _ (●ML ((Tl ++ [v]):list (leibnizO A)))
+           with "HTl") as "HTl".
+    { apply mono_list_update. by apply prefix_app_r. }
+    rewrite mono_list_auth_lb_op.
+    iDestruct "HTl" as "[HTl HTl']".
+    iAssert (frag_list χ Left n v) with "[HTl']" as "Hidx".
+    { iExists _. iFrame. iPureIntro. rewrite -Hvalid1.
+      rewrite lookup_app_r; [|lia]. rewrite minus_diag. done. }
+    rewrite Hvalid1.
+    iFrame "#∗".
+    iApply "Hclose".
+    iIntros "!>".
+    rewrite -drop_app_le; [|lia].
+    iExists (Tl ++ [v]), Tr, nl, nr.
+    rewrite app_length. rewrite Hvalid1. simpl.
+    replace (S n) with (n + 1)%nat by lia.
+    iFrame "#∗".
+    iSplit; iPureIntro; lia.
+  Qed.
+
+  Lemma step_update_send_r χ E n m pm v p :
+    ↑N ⊆ E →
+    ses_own χ Right n m (<!> pm)%proto -∗ iMsg_car pm v (Next p) -∗
+    |~{E}~> (ses_own χ Right (S n) m p ∗ ses_idx χ Right n v).
+  Proof.
+    iIntros (HE) "[#HI (Hp&HsrF&HrrF)] Hpm".
+    iApply step_update_open.
+    iInv N as "H" "Hclose".
+    iDestruct "H" as (Tl Tr nl nr)
+                       "(>%Hle&>%Hle2&Hctx&>HTl&>HTr&
+                       >Hsl&>Hrl&>Hsr&>Hrr&#>HTllb&#>HTrlb)".
+    iApply step_update_impl; [iApply step_update_lb_update; iApply "HTrlb"|].
+    iApply step_update_lb_step; [iApply "HTllb"|]=> /=.
+    iIntros "!>!>!>".
+    iMod (iProto_send_r with "Hctx Hp Hpm") as "[Hctx Hp]".
+    iModIntro.
+    iApply step_fupdN_intro; [done|].
+    iApply (bi.laterN_le (length (drop nr Tl))); [rewrite drop_length; lia|].
+    iIntros "!> #HTrlb'".
+    iDestruct (own_valid_2 with "Hsr HsrF") as %Hvalid1%excl_auth_agree_L.
+    iDestruct (own_valid_2 with "Hrr HrrF") as %Hvalid2%excl_auth_agree_L.
+    iMod (own_update_2 _ _ _ (●E (S (length Tr)) ⋅ ◯E (S (length Tr)))
+           with "Hsr HsrF") as "[Hsr HsrF]"; [by apply excl_auth_update|].
+    iMod (own_update _ _ (●ML ((Tr ++ [v]):list (leibnizO A)))
+           with "HTr") as "HTr".
+    { apply mono_list_update. by apply prefix_app_r. }
+    rewrite mono_list_auth_lb_op.
+    iDestruct "HTr" as "[HTr HTr']".
+    iAssert (frag_list χ Right n v) with "[HTr']" as "Hidx".
+    { iExists _. iFrame. iPureIntro. rewrite -Hvalid1.
+      rewrite lookup_app_r; [|lia]. rewrite minus_diag. done. }
+    rewrite !Hvalid1.
+    iFrame "#∗".
+    iApply "Hclose".
+    iIntros "!>".
+    rewrite -drop_app_le; [|lia].
+    iExists Tl, (Tr ++ [v]), nl, nr.
+    rewrite app_length.
+    iFrame "#∗".
+    rewrite Hvalid1. simpl. iFrame.
+    replace (S n) with (n + 1)%nat by lia.
+    iFrame "#∗".
+    iSplit; iPureIntro; lia.
+  Qed.
+
+  (* TODO: Unify the proof of the above rules into this one. *)
+  Lemma step_update_send χ s E n m pm v p :
+    ↑N ⊆ E →
+    ses_own χ s n m (<!> pm)%proto -∗ iMsg_car pm v (Next p) -∗
+    |~{E}~> (ses_own χ s (S n) m p ∗ ses_idx χ s n v).
+  Proof.
+    iIntros (HE) "Hp Hpm".
+    destruct s.
+    - by iApply (step_update_send_l with "Hp Hpm").
+    - by iApply (step_update_send_r with "Hp Hpm").
+  Qed.
+
+  Lemma step_update_recv_l χ E n m pm v :
+    ↑N ⊆ E →
+    ses_own χ Left n m (<?> pm)%proto -∗ ses_idx χ Right m v -∗
+    |~{E}~> ∃ p, ses_own χ Left n (S m) p ∗ iMsg_car pm v (Next p).
+  Proof.
+    iIntros (HE) "[#HI (Hp&HslF&HrlF)] Hidx".
+    iApply step_update_open.
+    iInv N as "H" "Hclose".
+    iDestruct "H" as (Tl Tr nl nr)
+                       "(>%Hle&>%Hle2&Hctx&>HTl&>HTr&
+                         >Hsl&>Hrl&>Hsr&>Hrr&#>HTllb&#>HTrlb)".
+    iDestruct (own_valid_2 with "Hrl HrlF") as %Hvalid%excl_auth_agree_L.
+    rewrite Hvalid.
+    iDestruct "Hidx" as (Tr') "[%Hlookup HTr']".
+    iDestruct (own_valid_2 with "HTr HTr'") as %Hvalid'%mono_list_both_valid_L.
+    destruct Hvalid' as [Tr'' ->].
+    assert (m < length Tr')%nat as Hm.
+    { by eapply (lookup_lt_Some Tr' m). }
+    rewrite drop_app_le; last first.
+    { by apply Nat.lt_le_incl. }
+    rewrite (drop_S Tr' v m); [|done]=> /=.
+    iApply step_update_lb_step; [iApply "HTrlb"|]=> /=.
+    assert (1 ≤ length Tr') by lia.
+    iFrame.
+    iIntros "!>!>!>".
+    iMod (iProto_recv_l with "Hctx Hp") as (p) "(Hctx & Hp &HP)".
+    iMod (own_update_2 _ _ _ (●E (S m) ⋅ ◯E (S m))
+           with "Hrl HrlF") as "[Hrl HrlF]"; [by apply excl_auth_update|].
+    iModIntro.
+    simpl.
+    destruct Tr' as [|r Tr']; [done|]=> /=.
+    iIntros "!>!>!>".
+    iApply step_fupdN_intro; [done|].
+    iIntros "!>".
+    iFrame.
+    iMod ("Hclose" with "[-Hp HP]") as "_".
+    { iNext. iExists Tl,((r::Tr')++Tr''),(S m),nr. iFrame "#∗".
+      rewrite drop_app_le; last first.
+      { apply lt_n_Sm_le, le_n_S. done. }
+      iFrame.
+      iSplit; iPureIntro.
+      - done.
+      - rewrite app_length.
+        etransitivity. apply Hm.
+        apply Nat.le_add_r. }
+    iModIntro. iFrame "#∗".
+    iExists p. iFrame.
+  Qed.
+
+  Lemma step_update_recv_r χ E n m pm v :
+    ↑N ⊆ E →
+    ses_own χ Right n m (<?> pm)%proto -∗ ses_idx χ Left m v -∗
+    |~{E}~> ∃ p, ses_own χ Right n (S m) p ∗ iMsg_car pm v (Next p).
+  Proof.
+    iIntros (HE) "[#HI (Hp&HsrF&HrrF)] Hidx".
+    iApply step_update_open.
+    iInv N as "H" "Hclose".
+    iDestruct "H" as (Tl Tr nl nr)
+                       "(>%Hle&>%Hle2&Hctx&>HTl&>HTr&
+                         >Hsl&>Hrl&>Hsr&>Hrr&#>HTllb&#>HTrlb)".
+    iDestruct (own_valid_2 with "Hrr HrrF") as %Hvalid%excl_auth_agree_L.
+    rewrite Hvalid.
+    iDestruct "Hidx" as (Tl') "[%Hlookup HTl']".
+    iDestruct (own_valid_2 with "HTl HTl'") as %Hvalid'%mono_list_both_valid_L.
+    destruct Hvalid' as [Tl'' ->].
+    assert (m < length Tl')%nat as Hm.
+    { by eapply (lookup_lt_Some Tl' m). }
+    rewrite drop_app_le; last first.
+    { by apply Nat.lt_le_incl. }
+    rewrite (drop_S Tl' v m); [|done]=> /=.
+    iApply step_update_lb_step; [iApply "HTllb"|]=> /=.
+    assert (1 ≤ length Tl') by lia.
+    iFrame.
+    iIntros "!>!>!>".
+    iMod (iProto_recv_r with "Hctx Hp") as (p) "(Hctx & Hp &HP)".
+    iMod (own_update_2 _ _ _ (●E (S m) ⋅ ◯E (S m))
+           with "Hrr HrrF") as "[Hrr HrrF]"; [by apply excl_auth_update|].
+    iModIntro.
+    simpl.
+    destruct Tl' as [|l Tl']; [done|]=> /=.
+    iIntros "!>!>!>".
+    iApply step_fupdN_intro; [done|].
+    iIntros "!>".
+    iFrame.
+    iMod ("Hclose" with "[-Hp HP]") as "_".
+    { iNext. iExists ((l::Tl')++Tl''),Tr,nl,(S m). iFrame "#∗".
+      rewrite drop_app_le; last first.
+      { apply lt_n_Sm_le, le_n_S. done. }
+      iFrame.
+      iSplit; iPureIntro.
+      - rewrite app_length.
+        etransitivity. apply Hm.
+        apply Nat.le_add_r.
+      - done. }
+    iModIntro. iFrame "#∗".
+    iExists p. iFrame.
+  Qed.
+
+  (* TODO: Unify the proof of the above rules into this one. *)
+  Lemma step_update_recv χ s E n m pm v :
+    ↑N ⊆ E →
+    ses_own χ s n m (<?> pm)%proto -∗ ses_idx χ (dual_side s) m v -∗
+    |~{E}~> ∃ p, ses_own χ s n (S m) p ∗ iMsg_car pm v (Next p).
+  Proof.
+    iIntros (HE) "Hp Hpm".
+    destruct s.
+    - by iApply (step_update_recv_l with "Hp Hpm").
+    - by iApply (step_update_recv_r with "Hp Hpm").
+  Qed.
+
+End iProto_sessions.
